lean/Spacewave.lean
@@ -3,5 +3,6 @@ import Spacewave.SObject.ConfigChain
 import Spacewave.SObject.Crypto
 import Spacewave.SObject.ResolvedOps
 import Spacewave.SObject.State
+import Spacewave.SObject.Host
 
 #assert_standard_axioms
